Added GhostSeq

theories/typing/refined.v
@@ -5,19 +5,55 @@ Set Default Proof Using "Type".
 
 Implicit Type 𝔄 𝔅 ℭ: syn_type.
 
+Section obs_def.
+Context `{!invGS Σ, !prophG Σ}.
+
+Definition proph_obs_s (φπ: proph Prop) : iProp Σ :=
+  proph_obs φπ ∗ ∃π, ⌜φπ π⌝.
+End obs_def.
+
+Notation ".⟨ φπ ⟩S" := (proph_obs_s φπ%type%stdpp)
+  (at level 1, format ".⟨ φπ ⟩S") : bi_scope.
+Notation "⟨ π , φ ⟩S" := (proph_obs_s (λ π, φ%type%stdpp))
+  (at level 1, format "⟨ π ,  φ ⟩S") : bi_scope.
+
+Section obs.
+Context `{!invGS Σ, !prophG Σ}.
+Global Instance proph_obs_s_persistent φπ : Persistent .⟨φπ⟩S := _.
+Global Instance proph_obs_s_timeless φπ : Timeless .⟨φπ⟩S := _.
+Global Instance proph_obs_s_proper :
+  Proper (pointwise_relation _ (↔) ==> (⊣⊢)) proph_obs_s.
+Proof. solve_proper. Qed.
+Global Instance proph_obs_s_mono :
+  Proper (pointwise_relation _ impl ==> (⊢)) proph_obs_s.
+Proof. solve_proper. Qed.
+
+Lemma proph_obs_s_impl (φπ ψπ: proph Prop) : (∀π, φπ π → ψπ π) → .⟨φπ⟩S -∗ .⟨ψπ⟩S.
+Proof. move=> Imp. do 2 f_equiv. move=> ?. by apply Imp. Qed.
+
+Lemma proph_obs_s_true (φπ: proph Prop) : (∀π, φπ π) → ⊢ .⟨φπ⟩S.
+Proof. iIntros. iSplit. by iApply proph_obs_true. iExists inhabitant. iPureIntro. done. Qed.
+
+Lemma proph_obs_upgrade E (φπ: proph Prop): ↑prophN ⊆ E → proph_ctx -∗ .⟨φπ⟩ ={E}=∗ .⟨φπ⟩S.
+Proof. 
+  iIntros (?) "PROPH #Obs". iMod (proph_obs_sat with "PROPH Obs") as "%"; [done|]. 
+  iModIntro. iFrame "Obs". done.
+Qed.
+End obs.
+
 Section refined.
   Context `{!typeG Σ}.
 
   Lemma split_mt_refined {𝔄} Φ (ty: type 𝔄) vπ d tid l :
-    (l ↦∗: λ vl, ⟨π, Φ (vπ π)⟩ ∗ ty.(ty_own) vπ d tid vl) ⊣⊢
-    ⟨π, Φ (vπ π)⟩ ∗ l ↦∗: ty.(ty_own) vπ d tid.
+    (l ↦∗: λ vl, ⟨π, Φ (vπ π)⟩S ∗ ty.(ty_own) vπ d tid vl) ⊣⊢
+    ⟨π, Φ (vπ π)⟩S ∗ l ↦∗: ty.(ty_own) vπ d tid.
   Proof. iSplit; [|iIntros "[$$]"]. iIntros "(%&?&$&?)". iExists _. iFrame. Qed.
 
   Program Definition refined {𝔄} (Φ: pred' 𝔄) (ty: type 𝔄) := {|
     ty_size := ty.(ty_size);  ty_lfts := ty.(ty_lfts);  ty_E := ty.(ty_E);
-    ty_proph := ty.(ty_proph);
-    ty_own vπ d tid vl := ⟨π, Φ (vπ π)⟩ ∗ ty.(ty_own) vπ d tid vl;
-    ty_shr vπ d κ tid l := ⟨π, Φ (vπ π)⟩ ∗ ty.(ty_shr) vπ d κ tid l;
+    ty_proph vπ ξl := ty.(ty_proph) vπ ξl /\ exists π, Φ (vπ π);
+    ty_own vπ d tid vl := ⟨π, Φ (vπ π)⟩S ∗ ty.(ty_own) vπ d tid vl;
+    ty_shr vπ d κ tid l := ⟨π, Φ (vπ π)⟩S ∗ ty.(ty_shr) vπ d κ tid l;
   |}%I.
   Next Obligation. iIntros "* [_ ?]". by rewrite ty_size_eq. Qed.
   Next Obligation. iIntros "*% [$?]". by iApply ty_own_depth_mono. Qed.
@@ -29,12 +65,16 @@ Section refined.
     by iApply (ty_share with "LFT In Bor κ").
   Qed.
   Next Obligation.
-    iIntros "*% LFT In [$ ty] κ". by iApply (ty_own_proph with "LFT In ty κ").
+    iIntros "*% LFT In [#Obs ty] κ". iFrame "Obs". iDestruct "Obs" as "(_&%)".
+    assert (∀ ξl, (ty.(ty_proph) vπ ξl /\ exists π, Φ (vπ π)) ↔ ty.(ty_proph) vπ ξl). intuition.
+    setoid_rewrite H1. by iApply (ty_own_proph with "LFT In ty κ").
   Qed.
   Next Obligation.
-    iIntros "*% LFT In In' [_ ty] κ". by iApply (ty_shr_proph with "LFT In In' ty κ").
+    iIntros "*% LFT In In' [[_ %] ty] κ".
+    assert (∀ ξl, (ty.(ty_proph) vπ ξl /\ exists π, Φ (vπ π)) ↔ ty.(ty_proph) vπ ξl). intuition.
+    setoid_rewrite H1. by iApply (ty_shr_proph with "LFT In In' ty κ").
   Qed.
-  Next Obligation. move=> *. by eapply ty_proph_weaken. Qed.
+  Next Obligation. move=> ?????[??]. by eapply ty_proph_weaken. Qed.
 
   Global Instance refined_ne {𝔄} (Φ: 𝔄 → _) : NonExpansive (refined Φ).
   Proof. solve_ne_type. Qed.
@@ -47,8 +87,8 @@ Section typing.
 
   Global Instance refined_type_ne {𝔄} (Φ: 𝔄 → _) : TypeNonExpansive !{Φ}%T.
   Proof.
-    split; [|split|..]=>/= *; [done| by apply type_lft_morphism_id_like|intuition| |by f_equiv..].
-    eexists [_], [_]. intuition. by constructor. by inversion_clear H.
+    split; [|split|..]=>/= *; [done| by apply type_lft_morphism_id_like|by f_equiv| |by f_equiv..].
+    eexists [_], [_]. intuition. by constructor. by inversion_clear H1.
   Qed.
 
   Global Instance refined_send {𝔄} (Φ: 𝔄 → _) ty : Send ty → Send (!{Φ} ty).
@@ -75,10 +115,12 @@ Section typing.
     subtype E L (!{Φ} ty) (!{Ψ} ty') f.
   Proof.
     iIntros (Sub Imp ?) "L". iDestruct (Sub with "L") as "#Sub".
-    iIntros "!> E". iDestruct ("Sub" with "E") as "(%&?& #InOwn & #InShr)".
-    do 2 (iSplit; [done|]).
+    iIntros "!> E". iDestruct ("Sub" with "E") as "((%&%)&?& #InOwn & #InShr)".
+    iSplit. iPureIntro. split; [done|].
+    intros ??(?&?&?). split. intuition. exists x. by apply Imp.
+    iSplit; [done|].
     iSplit; iIntros "!>*[??]"; iSplit; [|by iApply "InOwn"| |by iApply "InShr"];
-    (iApply proph_obs_impl; [|done]=>/= ?; apply Imp).
+    (iApply proph_obs_s_impl; [|done]=>/= ?; apply Imp).
   Qed.
   Lemma refined_eqtype {𝔄 𝔅} (Φ Ψ: _ → Prop) (f: 𝔄 → 𝔅) g ty ty' E L :
     eqtype E L ty ty' f g → (∀a, Φ a → Ψ (f a)) → (∀a, Ψ a → Φ (g a)) →
@@ -87,11 +129,12 @@ Section typing.
 
   Lemma refined_forget {𝔄} (Φ: 𝔄 → _) ty E L : subtype E L (!{Φ} ty) ty id.
   Proof.
-    iIntros "% _!>_". iSplit; [done|]. iSplit; [by iApply lft_incl_refl|].
-    iSplit; iIntros "!>* [_$]".
+    iIntros "% _!>_". iSplit. iPureIntro. split; [done|].
+    intros ??(?&?&?). done.
+    iSplit; [by iApply lft_incl_refl|]. iSplit; iIntros "!>* [_$]".
   Qed.
 
-  Lemma refined_blocked_subtype {𝔄 𝔅} (Φ Ψ: _ → Prop) (f: 𝔄 → 𝔅) ty ty' :
+  (* Lemma refined_blocked_subtype {𝔄 𝔅} (Φ Ψ: _ → Prop) (f: 𝔄 → 𝔅) ty ty' :
     blocked_subtype ty ty' f →
     blocked_subtype (!{Φ} ty) (!{Ψ} ty') f.
   Proof. done. Qed.
@@ -100,18 +143,19 @@ Section typing.
     blocked_eqtype (!{Φ} ty) (!{Ψ} ty') f g.
   Proof. done. Qed.
   Lemma refined_blocked_forget {𝔄} (Φ: 𝔄 → _) ty : blocked_eqtype (!{Φ} ty) ty id id.
-  Proof. apply blocked_eqtype_unfold. apply _. done. Qed.
+  Proof. apply blocked_eqtype_unfold. apply _. done. Qed. *)
 
   Lemma tctx_refined_in {𝔄 𝔅l} (Φ: 𝔄 → _) ty E L (T: tctx 𝔅l) p :
     tctx_incl E L (p ◁ ty +:: T) (p ◁ !{Φ} ty +:: T)
       (λ post '(a -:: bl), Φ a ∧ post (a -:: bl)).
   Proof.
     split. { move=>/= ???[??]. by f_equiv. }
-    iIntros (??[??]?) "_ _ _ _ $ /=[(%&%&%& ⧖ & ty) T] Obs !>".
+    iIntros (??[??]?) "_ PROPH _ _ $ /=[(%&%&%& ⧖ & ty) T] #Obs".
+    iMod (proph_obs_upgrade with "PROPH Obs") as "ObsS"; [done|]. iModIntro.
     iExists (_-::_). iFrame "T". iSplit; last first.
     { by iApply proph_obs_impl; [|done]=>/= ?[_ ?]. }
     iExists _, _. iSplit; [done|]. iFrame "⧖ ty".
-    by iApply proph_obs_impl; [|done]=>/= ?[? _].
+    by iApply proph_obs_s_impl; [|done]=>/= ?[? _].
   Qed.
 
   Lemma tctx_refined_out {𝔄 𝔅l} (Φ: 𝔄 → _) ty E L (T: tctx 𝔅l) p :
@@ -119,7 +163,7 @@ Section typing.
       (λ post '(a -:: bl), Φ a → post (a -:: bl)).
   Proof.
     split. { move=>/= ???[??]. by apply forall_proper=> ?. }
-    iIntros (??[??]?) "_ _ _ _ $ /=[(%&%&%&?& Obs &?) T] Obs' !>".
+    iIntros (??[??]?) "_ _ _ _ $ /=[(%&%&%&?& [Obs _] &?) T] Obs' !>".
     iCombine "Obs Obs'" as "Obs". iExists (_-::_). iFrame "T".
     iSplit. { iExists _, _. by iFrame. }
     iApply proph_obs_impl; [|done]=>/= ?[? Imp]. by apply Imp.
@@ -130,12 +174,13 @@ Section typing.
       (λ post '(a -:: bl), Φ a ∧ post (a -:: bl)).
   Proof.
     split. { move=>/= ???[??]. by f_equiv. }
-    iIntros (??[??]?) "_ _ _ _ $ /=[p T] Obs".
+    iIntros (??[??]?) "_ PROPH _ _ $ /=[p T] #Obs".
+    iMod (proph_obs_upgrade with "PROPH Obs") as "ObsS"; [done|].
     iDestruct "p" as ([[]|][|]?) "[⧖ own]"=>//. iDestruct "own" as "[(%& >↦ & ty) †]".
     iModIntro. iExists (_-::_). iFrame "T". iSplit; last first.
     { by iApply proph_obs_impl; [|done]=>/= ?[_ ?]. }
     iExists _, _. iSplit; [done|]. iFrame "⧖ †". iNext. iExists _.
-    iFrame "↦ ty". by iApply proph_obs_impl; [|done]=>/= ?[? _].
+    iFrame "↦ ty". by iApply proph_obs_s_impl; [|done]=>/= ?[? _].
   Qed.
 
   Lemma tctx_own_refined_out {𝔄 𝔅l} (Φ: 𝔄 → _) ty n E L (T: tctx 𝔅l) p :
@@ -145,7 +190,7 @@ Section typing.
     split. { move=>/= ???[??]. by apply forall_proper=> ?. }
     iIntros (??[??]?) "_ _ _ _ $ /=[p T] Obs'".
     iDestruct "p" as ([[]|][|]?) "[⧖ own]"=>//.
-    iDestruct "own" as "[(%& >↦ & >Obs & ty) †]". iCombine "Obs Obs'" as "Obs".
+    iDestruct "own" as "[(%& >↦ & >[Obs _] & ty) †]". iCombine "Obs Obs'" as "Obs".
     iModIntro. iExists (_-::_). iFrame "T". iSplit; last first.
     { iApply proph_obs_impl; [|done]=>/= ?[? Imp]. by apply Imp. }
     iExists _, _. iSplit; [done|]. iFrame "⧖ †". iNext. iExists _. iFrame.
@@ -156,11 +201,12 @@ Section typing.
       (λ post '(a -:: bl), Φ a ∧ post (a -:: bl)).
   Proof.
     split. { move=>/= ???[??]. by f_equiv. }
-    iIntros (??[??]?) "_ _ _ _ $ /=[p T] Obs".
+    iIntros (??[??]?) "_ PROPH _ _ $ /=[p T] #Obs".
+    iMod (proph_obs_upgrade with "PROPH Obs") as "ObsS"; [done|].
     iDestruct "p" as ([[]|][|]?) "[⧖ ty]"=>//. iModIntro. iExists (_-::_).
     iFrame "T". iSplit; last first. { by iApply proph_obs_impl; [|done]=>/= ?[_ ?]. }
     iExists _, _. iSplit; [done|]. iFrame "⧖ ty".
-    by iApply proph_obs_impl; [|done]=>/= ?[? _].
+    by iApply proph_obs_s_impl; [|done]=>/= ?[? _].
   Qed.
 
   Lemma tctx_shr_refined_out {𝔄 𝔅l} (Φ: 𝔄 → _) ty κ E L (T: tctx 𝔅l) p :
@@ -169,7 +215,7 @@ Section typing.
   Proof.
     split. { move=>/= ???[??]. by apply forall_proper=> ?. }
     iIntros (??[??]?) "_ _ _ _ $ /=[p T] Obs'".
-    iDestruct "p" as ([[]|][|]?) "[⧖ shr]"=>//. iDestruct "shr" as "[Obs ty]".
+    iDestruct "p" as ([[]|][|]?) "[⧖ shr]"=>//. iDestruct "shr" as "[[Obs _] ty]".
     iCombine "Obs Obs'" as "Obs". iModIntro. iExists (_-::_). iFrame "T".
     iSplit. { iExists _, _. iSplit; [done|]. by iFrame. }
     iApply proph_obs_impl; [|done]=>/= ?[? Imp]. by apply Imp.
