theories/typing/lib/ghostptrtoken/ghostseq_basic.v
@@ -1,0 +1,205 @@
+From lrust.typing Require Export type.
+From lrust.typing Require Import array_util typing zst.
+From lrust.typing.lib.ghostptrtoken Require Import ghostseq.
+Set Default Proof Using "Type".
+
+Open Scope nat.
+Implicit Type 𝔄 𝔅: syn_type.
+
+Section ghostseq_basic.
+  Context `{!typeG Σ}.
+
+  Lemma real_big_sepL'_ty_shr {𝔄 𝔅} (ty: type 𝔄) (f: 𝔄 → 𝔅)
+    aπl (d: nat) κ tid l E L F q :
+    real E L ty f → ↑lftN ⊆ F → lft_ctx -∗ elctx_interp E -∗ llctx_interp L q -∗
+    ([∗ list] aπ ∈ aπl, ty.(ty_shr) aπ d κ tid l)
+      ={F}▷=∗ |={F}▷=>^d |={F}=>
+        ⌜∃bm, (fmap f) ∘ lapply aπl = const bm⌝ ∗ llctx_interp L q ∗
+        [∗ list] aπ ∈ aπl, ty.(ty_shr) aπ d κ tid l.
+  Proof.
+    iIntros ([_ Rl]?) "#LFT #E L tys". iInduction aπl as [|?] "IH" forall (q)=>/=.
+    { iApply step_fupdN_full_intro. iFrame "L". iPureIntro. unfold compose. by exists []. }
+    iDestruct "tys" as "[ty tys]". iDestruct "L" as "[L L₊]".
+    iMod (Rl with "LFT E L ty") as "Upd"; [done|].
+    iMod ("IH" with "L₊ tys") as "Upd'". iCombine "Upd Upd'" as "Upd". iIntros "!>!>".
+    iApply (step_fupdN_wand with "Upd"). iIntros "[>(%Eq &$&$) >(%Eq' &$&$)] !%".
+    move: Eq=> [b Eq]. move: Eq'=> [bm Eq']. exists (b :: bm).
+    fun_ext=>/= π. by move: (equal_f Eq π) (equal_f Eq' π)=>/= <-<-.
+  Qed.
+
+  Global Instance seq_type_ne 𝔄 : TypeNonExpansive (ghostseq_ty (𝔄:=𝔄)).
+  Proof.
+    split; [done|split| |]; simpl.
+    - by apply type_lft_morphism_id_like.
+    - intros. do 6 f_equiv. intros ?. by eapply Forall2_impl.
+    - intros ???(?&?&->&->&?). eexists _, _. split. exact H. 
+      intros. eexists _, _. done.  
+    - intros **. by do 6 (f_contractive || f_equiv).
+    - intros **. by do 6 (f_contractive || f_equiv).
+  Qed.
+
+  Global Instance seq_send {𝔄} (ty: type 𝔄) : Send ty → Send (ghostseq_ty ty).
+  Proof.  move=> ?>/=. by do 6 (f_equiv || move=>?). Qed.
+
+  Global Instance seq_sync {𝔄} (ty: type 𝔄) : Sync ty → Sync (ghostseq_ty ty).
+  Proof. move=> ?>/=. by do 6 (f_equiv || move=>?). Qed.
+
+  Lemma seq_resolve {𝔄} (ty: type 𝔄) Φ E L :
+    resolve E L ty Φ → resolve E L (ghostseq_ty ty) (lforall Φ).
+  Proof.
+    iIntros (????????) "#LFT #PROPH #E L token //=".
+    iDestruct "token" as (?[->->]) "tys".
+    rewrite trans_big_sepL'_mt_ty_own.
+    iMod (resolve_big_sepL_ty_own with "LFT PROPH E L tys") as "Upd"; [done..|].
+    iApply (step_fupdN_wand with "Upd").
+    rewrite vec_to_list_to_vec. unfold lapply. setoid_rewrite lforall_Forall.
+    setoid_rewrite Forall_fmap. by iIntros "!> H".
+  Qed.
+
+  Lemma seq_resolve_just {𝔄} (ty: type 𝔄) E L :
+    resolve E L ty (const True) → resolve E L (ghostseq_ty ty) (const True).
+  Proof. move=> ?. apply resolve_just. Qed.
+
+  Lemma seq_real {𝔄 𝔅} (ty: type 𝔄) (f: 𝔄 → 𝔅) E L :
+    real E L ty f → real (𝔅:=listₛ _) E L (ghostseq_ty ty) (fmap f).
+  Proof.
+    move=> Rl. split; iIntros (????) "*% LFT E L token //=".
+    - iDestruct "token" as (?[->->]) "tys".
+      rewrite trans_big_sepL'_mt_ty_own.
+      iMod (real_big_sepL_ty_own with "LFT E L tys") as "Upd"; [done..|].
+      iApply (step_fupdN_wand with "Upd"). iIntros "!> >(%Eq &$&?) !>".
+      iSplit; last first.
+      { iExists _. iSplit; [done|].
+        rewrite trans_big_sepL'_mt_ty_own.  iFrame. }
+      iPureIntro. move: Eq=> [bl Eq]. exists (vec_to_list bl). fun_ext=>/= π.
+      move: (equal_f Eq π)=>/= <-.
+      rewrite 2! vec_to_list_map vec_to_list_to_vec -list_fmap_compose. reflexivity.
+    - iDestruct "token" as (?) "[%Bor tys]".
+      iMod (real_big_sepL'_ty_shr with "LFT E L tys") as "Upd"; [done..|].
+      iIntros "!>!>". iApply (step_fupdN_wand with "Upd").
+      iIntros ">(%Eq &$& tys) !>". iSplit; [|iExists _; by iFrame].
+      iPureIntro. move: Eq=> [bl Eq]. exists bl. fun_ext=>/= π.
+      move: (equal_f Eq π)=>/= <-.  by rewrite Bor.
+  Qed.
+
+  Lemma seq_subtype {𝔄 𝔅} (f: 𝔄 → 𝔅) ty ty' E L :
+    subtype E L ty ty' f → subtype E L (ghostseq_ty ty) (ghostseq_ty ty') (fmap f).
+  Proof.
+    iIntros (Sub ?) "L". iDestruct (Sub with "L") as "#Sub". iIntros "!> E".
+    iDestruct ("Sub" with "E") as "((%EqSz&%Proph) &?&#Own&#Shr)".
+    have Eq: ∀(aπl: list (proph 𝔄)), fmap f ∘ lapply aπl = lapply (fmap (f ∘.) aπl).
+    { move=> ?. fun_ext=>/= ?. rewrite /lapply -2!list_fmap_compose. reflexivity. }
+    iSplit. iPureIntro. split; [done|]. intros ??(?&?&->&->&?).
+    rewrite Eq. eexists _, _. do 2 (split; [done|]). rewrite Forall2_fmap_l.
+    eapply Forall2_impl. done. simpl. intros. by apply Proph.
+    iSplit; [done|]. iSplit; iIntros "!>" (??) "* token //=".
+    - iDestruct "token" as (?[->->]) "tys". iExists  _.
+      iSplit; [done|]. rewrite big_opL_fmap. simpl.
+      iApply (big_sepL_impl with "[$]");
+      iModIntro; iIntros (???). simpl. iApply "Own".
+    - iDestruct "token" as (?->) "↦". iExists _. rewrite Eq.
+      iSplit; [done|].
+      rewrite big_opL_fmap. iApply (big_sepL_impl with "↦").
+      iModIntro. iIntros (???). iApply "Shr".
+  Qed.
+  Lemma seq_eqtype {𝔄 𝔅} (f: 𝔄 → 𝔅) g ty ty' E L :
+    eqtype E L ty ty' f g → eqtype E L (ghostseq_ty ty) (ghostseq_ty ty') (fmap f) (fmap g).
+  Proof. move=> [??]. split; by apply seq_subtype. Qed.
+
+  Global Instance seq_zst {𝔄} (ty: type 𝔄) : ZST (ghostseq_ty ty).
+  Proof. done. Qed.
+
+  Lemma seq_append {𝔄} (ty: type 𝔄) E L :
+  tctx_incl E L +[null_val ◁ (box (ghostseq_ty ty)); null_val ◁ (box (ghostseq_ty ty))] +[null_val ◁ (box (ghostseq_ty ty))]
+    (λ post '-[s1; s2], post -[s1 ++ s2]).
+  Proof. split. solve_proper.
+    iIntros (??(s1π&s2π&[])?) "_ _ _ _ $ (ty1&ty2&true) Obs"; 
+    iExists (-[λ π, _]); iFrame.
+    rewrite 3! tctx_elt_interp_zst.
+    iDestruct "ty1" as "(%&⧖&%&>(_&->)&ty1)".
+    iDestruct "ty2" as "(%&⧖'&%&>(_&->)&ty2)".
+    iCombine "⧖ ⧖'" as "⧖". simpl.
+    iModIntro. iExists _. iFrame. iNext. iExists _.
+    iSplit. iPureIntro. split; [done|]. fun_ext. intros. rewrite -fmap_app. done.
+    rewrite big_sepL_app. iSplitL "ty1"; 
+    (iApply (big_sepL_impl with "[-]"); [done|]); iIntros "!> **";
+    (iApply ty_own_depth_mono; [|done]); lia.
+  Qed.
+
+  Lemma seq_new {𝔄} (ty: type 𝔄) E L :
+  tctx_incl E L +[null_val ◁ (box ())] +[null_val ◁ (box (ghostseq_ty ty))]
+    (λ post '-[_], post -[[]]).
+  Proof. split. solve_proper.
+    iIntros (??(?&[])?) "_ _ _ _ $ (⧖&true) Obs"; 
+    iExists (-[λ π, _]); iFrame.
+    rewrite tctx_elt_interp_zst tctx_hasty_val.
+    iDestruct "⧖" as ([|?]) "(⧖&?)"; [done|].
+    iModIntro. iExists _. iFrame. iNext. iExists []. iSplit; done.
+  Qed.
+
+  (* Lemma seq_split {𝔄 𝔄l} (ty: type 𝔄) `{!Copy ty} (T: tctx 𝔄l) E L :
+  tctx_incl E L (null_val ◁ (box (ghostseq_ty ty)) +:: T) (null_val ◁ (box (ghostseq_ty ty)) +:: null_val ◁ (box (ghostseq_ty ty)) +:: T)
+    (λ post '(s -:: al), ∃ s1 s2, s1 ++ s2 = s ∧ post (s1 -:: s2 -:: al)).
+  Proof. split. solve_proper.
+    iIntros (??(sπ&lπ)?) "_ PROPH _ _ $ (ty&?) Obs".
+    rewrite tctx_elt_interp_zst.
+    iDestruct "ty" as "(%&⧖&%&>(_&->)&ty1)".
+    iMod (proph_obs_sat with "PROPH Obs") as "(%&%&%&%&%)"; [done|].
+    iExists ((λ π, _) -:: lπ); iFrame. *)
+    
+    
+    (* iDestruct "ty2" as "(%&⧖'&%&>(_&->)&ty2)".
+    iCombine "⧖ ⧖'" as "⧖". simpl.
+    iModIntro. iExists _. iFrame. iNext. iExists _.
+    iSplit. iPureIntro. split; [done|]. fun_ext. intros. rewrite -fmap_app. done.
+    rewrite big_sepL_app. iSplitL "ty1"; 
+    (iApply (big_sepL_impl with "[-]"); [done|]); iIntros "!> **";
+    (iApply ty_own_depth_mono; [|done]); lia.
+  Qed. *)
+
+  Lemma seq_one `{!Inhabited 𝔄} (ty: type 𝔄) `{!ZST ty} E L : eqtype E L (!{λ (l: listₛ 𝔄), length l = 1} (ghostseq_ty ty)) ty (λ (l: list 𝔄), l !!! 0) (λ x, [x]).
+  Proof. 
+    split; iIntros; iModIntro; iIntros "_".
+    - iSplit. iPureIntro. split. rewrite zero_size. done.
+      intros ??(([|?[|]]&?&->&->&?)&?&?); try done. 
+      inversion_clear H. inversion_clear H2. simpl. rewrite right_id. done.
+      iSplit. iApply lft_incl_refl.
+      iSplit; iModIntro; iIntros (????); [|iIntros (?)]; iIntros "((_&%&%)&%&%&ty)"; [destruct H0 as [->->]| revert H0; intros ->];
+      destruct aπl as [|?[|]]; try done; iDestruct "ty" as "(?&_)"; iFrame. 
+    - iSplit. iPureIntro. split. rewrite zero_size. done.
+      intros. simpl. split. exists [vπ], [ξl]. simpl. rewrite right_id. intuition. 
+      exists inhabitant. done.
+      iSplit. iApply lft_incl_refl.
+      iSplit; iModIntro; iIntros; (iSplit; [by iApply proph_obs_s_true|]); iExists [vπ];
+      [iDestruct (zst_size_eq with "[$]") as %->|]; simpl; (iSplit; [done|]); iSplit; done.
+  Qed.
+
+  (* Lemma seq_perm {𝔄}  g ty E L :
+   (∀ x, f x ≡ₚ x) → subtype E L (ghostseq_ty ty) (ghostseq_ty ty) f.
+  Proof. move=> [??]. split; by apply seq_subtype. Qed. *)
+
+  (* Rust's GhostSeq::new *)
+  Definition ghostseq_new: val :=
+    fn: [] :=
+      let: "r" := new [ #0] in
+      return: ["r"].
+
+  Lemma ghostseq_new_type {𝔄} (ty: type 𝔄) :
+    typed_val ghostseq_new (fn(∅) → ghostseq_ty ty) (λ post _, post []).
+  Proof.
+    eapply type_fn; [apply _|]=> _ ???. simpl_subst.
+    iIntros (???) "_ #TIME _ _ _ Na L C _ Obs". iMod persistent_time_receipt_0 as "⧖".
+    wp_bind (new _). iApply (wp_persistent_time_receipt with "TIME ⧖"); [done|].
+    iApply wp_new; [done..|]. iIntros "!>" (l) "[† _] ⧖". wp_seq.
+    do 2 wp_seq.
+    rewrite cctx_interp_singleton.
+    iApply ("C" $! [# #_] -[const []] with "Na L [-Obs] Obs"). iSplit; [|done].
+    iExists _, _. do 2 (iSplit; [done|]). rewrite/= freeable_sz_full split_mt_seq. 
+    iFrame "†". iNext. iExists []. iSplit.
+    iPureIntro. done.
+    rewrite heap_mapsto_vec_nil. iSplit; done.
+  Qed.
+End ghostseq_basic.
+
+Global Hint Resolve seq_resolve | 5 : lrust_typing.
+Global Hint Resolve seq_resolve_just seq_subtype seq_eqtype : lrust_typing.
